some more work on improved sequencing

CPS_Ctl/Seq.thy
@@ -39,11 +39,98 @@ definition seq_sem_l :: "syn \<Rightarrow> 'x state \<Rightarrow> 'x state" wher
   seq_sem_lifting
   seq_sem'"
 
-
-definition seq_sem :: "(syn, 'x state) sem" where
+definition seq_sem :: "(syn, 'x, 'x state) sem" where
 "seq_sem \<equiv>
   \<lparr> s_sem = seq_sem_l
   , s_cont = 
     LOut (seq_sem_lifting) Sseq \<rparr>"
 
+definition seq_sem_l_gen ::
+  "('s \<Rightarrow> syn) \<Rightarrow>
+   (syn, 'x state', ('y :: Pord)) lifting \<Rightarrow>
+   's \<Rightarrow> 'y \<Rightarrow> 'y" where
+"seq_sem_l_gen lfts lft =
+  lift_map_s lfts
+  lft
+  seq_sem'"
+
+(* TODO: the next thing is making
+   sure this all still works in the face of a true merge
+   with multiple liftings. *)
+definition seq_semx :: 
+"('s \<Rightarrow> syn) \<Rightarrow>
+ (syn, 'x state', ('y :: Pord)) lifting \<Rightarrow>
+ ('s, 'x, ('y :: Pord)) sem" where
+"seq_semx lfts lft \<equiv>
+  \<lparr> s_sem = seq_sem_l_gen lfts lft
+  , s_cont =
+    LOut lft Sseq \<rparr>"
+  
+
+(* 
+  question
+    - is it enough to say "we have a GS that extends Seq"
+    - do we need to account for multiple "layers" of composition?
+
+    - if we have a big compound, we would need a bunch of
+GS, one for each sub-language
+    - type parameter (local syntax) would vary
+    - 
+*)
+
+lemma HSeq :
+  assumes HV : "lifting_valid_weak lft Sv"
+  assumes H0 : "gs = seq_semx lfts lft"
+  assumes H1 : "lfts Sseq' = Sseq"
+  assumes H : "|gs| {- P1 -} cs {- P2 -}"
+  shows "|gs| {- P1 -} [G Sseq' cs] {- P2 -}"
+proof
+  fix c'
+  assume Safe : "|gs| {P2} c'"
+
+  have Guarded : "|gs| {P1} cs @ c'"
+    using HTE[OF H Safe]
+    by auto
+
+  show "|gs| {P1} [G Sseq' cs] @ c'"
+  proof
+    fix m
+    assume M : "P1 m"
+    assume CM : "s_cont gs m = [G Sseq' cs] @ c'"
+
+    obtain m1 where
+      Step : "sem_step_p gs m m1" and
+      CM1 : "s_cont gs m1 = cs @ c'"
+      using CM lifting_valid_weakDO[OF HV] unfolding H0
+      by(simp add: sem_step_p_eq sem_step_def seq_semx_def seq_sem_l_gen_def seq_sem'_def H1)
+
+
+    have M1_eq : "LUpd lft Sseq (cs @ c') m = m1" using Step CM H1 unfolding sem_step_p_eq H0 CM
+      by(simp add: sem_step_p_eq sem_step_def seq_semx_def seq_sem_l_gen_def seq_sem'_def split: option.splits list.splits)
+
+    (* need to put entire lifting into definition *)
+    have M1 : "P1 m1" sorry
+
+    have Conc' : "safe gs m1" using guardedD[OF Guarded M1 CM1]
+      by auto
+
+    show "safe gs m"
+    proof
+      fix m'
+      assume XP : "sem_exec_p gs m m'"
+        
+      show "imm_safe gs m'" using XP unfolding sem_exec_p_def
+      proof(cases rule: rtranclp.cases)
+      case rtrancl_refl
+        then show ?thesis using imm_safeI_Step[OF Step] by auto
+      next
+        case RT : (rtrancl_into_rtrancl b)
+
+        have Exc : "sem_exec_p gs m1 m'" unfolding sem_exec_p_def using rtranclp_bisect1[OF sem_step_determ RT(1) Step RT(2)] by auto
+
+        then show ?thesis using safeD[OF Conc' Exc] by auto
+      qed
+    qed
+  qed
+qed
 end
