Hoare/CPS_Hoare.thy
@@ -29,31 +29,29 @@ fun s_error_safe :: "s_error \<Rightarrow> bool" where
 record ('syn, 'mstate) sem' =
   s_sem :: "'syn \<Rightarrow> 'mstate \<Rightarrow> 'mstate"
 
-(* TODO: list updates *)
-record ('syn, 'mstate) sem = "('syn, 'mstate) sem'" +
-  s_cont :: "'mstate \<Rightarrow> 'syn gensyn list"
+(* TODO: this should be an entire lifting (at least a weak lifting.) *)
+record ('syn, 'full, 'mstate) sem = "('syn, 'mstate) sem'" +
+  s_cont :: "'mstate \<Rightarrow> 'full gensyn list"
 
-(* OK, for CPS approach we need to have each control-flow state
-   be able to manipulate and return a list of targets *)
+definition close :: "('syn, 'full, 'mstate) sem \<Rightarrow> ('full \<Rightarrow> 'syn) \<Rightarrow> ('full, 'full, 'mstate) sem" where
+"close s f =
+  \<lparr> s_sem = (s_sem s o f)
+  , s_cont = s_cont s \<rparr>"
 
-
-(* where is path update *)
-
-(* need to deal with this difference around halting behavior. *)
-(*
-definition sem_step ::
-  "('x, 'mstate) sem \<Rightarrow>
-   'mstate \<Rightarrow>
-   ('mstate * 'x s_error)" where
-"sem_step gs m =
-  (case s_next gs m of
-    Done \<Rightarrow> (m, Halted)
-    | Exec sub \<Rightarrow> (s_sem gs sub m, Exec sub)
-    | f \<Rightarrow> (m, f))"
+(* "closed" sem
+   we obtain this when our "full" syntax becomes the same as
+   our "individual syntax"
 *)
+type_synonym ('syn, 'mstate) semc = "('syn, 'syn, 'mstate) sem"
+
+record ('syn, 'full, 'mstate) semt = "('syn, 'full, 'mstate) sem" +
+  s_transl :: "'full \<Rightarrow> 'syn"
+
+definition s_semt :: "('syn, 'full, 'mstate) semt \<Rightarrow> 'full \<Rightarrow> 'mstate \<Rightarrow> 'mstate" where
+"s_semt s = s_sem s o s_transl s"
 
 definition sem_step ::
-  "('x, 'mstate) sem \<Rightarrow>
+  "('syn, 'mstate) semc \<Rightarrow>
    'mstate \<Rightarrow>
    ('mstate option)" where
 "sem_step gs m =
@@ -67,9 +65,8 @@ see if this will break any typeclasses...
 
 *)
 
-(* maybe use a relational small-step, relate it to the executable one? *)
 fun sem_exec ::
-  "('x, 'mstate) sem \<Rightarrow>
+  "('x, 'mstate) semc \<Rightarrow>
    nat \<Rightarrow>
    'mstate \<Rightarrow>
    ('mstate * s_error)" where
@@ -83,7 +80,7 @@ fun sem_exec ::
     | ((G x l)#tt) \<Rightarrow> sem_exec gs n (s_sem gs x m))"
 
 inductive sem_step_p ::
-  "('x, 'mstate) sem \<Rightarrow> 'mstate \<Rightarrow> 'mstate \<Rightarrow> bool"
+  "('x, 'mstate) semc \<Rightarrow> 'mstate \<Rightarrow> 'mstate \<Rightarrow> bool"
   where
 "\<And> gs (m :: 'mstate) (m' :: 'mstate) x l  tt .
  s_cont gs m = ((G x l)#tt) \<Longrightarrow> 
@@ -91,9 +88,11 @@ inductive sem_step_p ::
  sem_step_p gs m m'"
 
 definition sem_exec_p ::
-  "('x, 'mstate) sem \<Rightarrow> 'mstate \<Rightarrow> 'mstate \<Rightarrow> bool" where
+  "('x, 'mstate) semc \<Rightarrow> 'mstate \<Rightarrow> 'mstate \<Rightarrow> bool" where
 "sem_exec_p gs \<equiv>
   (rtranclp (sem_step_p gs))"
+
+declare sem_exec_p_def [simp add]
 
 lemma sem_step_p_sem_step :
   assumes H : "sem_step_p gs m m'"
@@ -109,6 +108,11 @@ lemma sem_step_sem_step_p :
   shows "sem_step_p gs m m'" using H
   by(auto simp add: sem_step_def split: s_error.splits list.splits option.splits intro: sem_step_p.intros)
 
+lemma sem_step_p_eq :
+  "(sem_step_p gs m m') = (sem_step gs m = Some m') "
+  using sem_step_p_sem_step sem_step_sem_step_p
+  by auto
+
 lemma sem_step_exec1 :
   assumes H : "sem_step gs m = Some m'"
   shows "\<exists> s . (sem_exec gs 1 m = (m', s))" using H
@@ -120,43 +124,81 @@ lemma sem_exec1_step :
   shows "sem_step gs m = Some m'" using assms
   by(auto simp add: sem_step_def split:option.splits list.splits)
 
-(*
-lemma sem_exec_snd :
-  assumes H : "sem_exec gs n m = (m', x)"
-  shows "x = s_next gs m'" using assms
-proof(induction n arbitrary: m m' x)
-  case 0
-  then show ?case by auto
-next
-  case (Suc n)
-  then show ?case 
-    apply(auto split: s_error.splits)
-qed
-*)
-
 (* have the state contain a delta to the continuation list?
    that is, a new prefix to prepend *)
-definition imm_safe :: "('x, 'mstate) sem \<Rightarrow> 'mstate \<Rightarrow> bool" where
+definition imm_safe :: "('x, 'mstate) semc \<Rightarrow> 'mstate \<Rightarrow> bool" where
 "imm_safe gs m \<equiv>
  ((s_cont gs m = []) \<or>
   (\<exists> m' . sem_step_p gs m m'))"
 
-definition safe :: "('x, 'mstate) sem \<Rightarrow> 'mstate \<Rightarrow> bool" where
+lemma imm_safeI_Done :
+  assumes H : "s_cont gs m = []"
+  shows "imm_safe gs m" using H
+  unfolding imm_safe_def by auto
+
+lemma imm_safeI_Step :
+  assumes H : "sem_step_p gs m m'"
+  shows "imm_safe gs m" using H
+  unfolding imm_safe_def by auto
+
+lemma imm_safeD :
+  assumes H : "imm_safe gs m"
+  shows "((s_cont gs m = []) \<or>
+  (\<exists> m' . sem_step_p gs m m'))" using H
+  unfolding imm_safe_def by auto
+
+
+definition safe :: "('x, 'mstate) semc \<Rightarrow> 'mstate \<Rightarrow> bool" where
 "safe gs m \<equiv>
   (\<forall> m' . sem_exec_p gs m m' \<longrightarrow> imm_safe gs m')"
 
+lemma safeI [intro]:
+  assumes H : "\<And> m' . sem_exec_p gs m m' \<Longrightarrow> imm_safe gs m'"
+  shows "safe gs m" using H unfolding safe_def
+  by auto
+
+lemma safeD :
+  assumes H : "safe gs m"
+  assumes Hx : "sem_exec_p gs m m'"
+  shows "imm_safe gs m'" using H Hx
+  unfolding safe_def by auto
+
 (* TODO: syntax *)
-definition guarded :: "('x, 'mstate) sem \<Rightarrow> ('mstate \<Rightarrow> bool) \<Rightarrow> 'x gensyn list \<Rightarrow> bool"
+definition guarded :: "('x, 'mstate) semc \<Rightarrow> ('mstate \<Rightarrow> bool) \<Rightarrow> 'x gensyn list \<Rightarrow> bool"
 ("|_| {_} _")
  where
 "guarded gs P c =
   (\<forall> m . P m \<longrightarrow> s_cont gs m = c \<longrightarrow> safe gs m)"
 
-definition HT :: "('x, 'mstate) sem \<Rightarrow> ('mstate \<Rightarrow> bool) \<Rightarrow> 'x gensyn list \<Rightarrow> ('mstate \<Rightarrow> bool) \<Rightarrow> bool" 
+lemma guardedI [intro] :
+  assumes H : "\<And> m . P m \<Longrightarrow> s_cont gs m = c \<Longrightarrow> safe gs m"
+  shows "guarded gs P c" using H
+  unfolding guarded_def by auto
+
+lemma guardedD :
+  assumes H : "guarded gs P c"
+  assumes HP : "P m"
+  assumes Hcont : "s_cont gs m = c"
+  shows "safe gs m" using assms
+  unfolding guarded_def by auto
+
+definition HT :: "('x, 'mstate) semc \<Rightarrow> ('mstate \<Rightarrow> bool) \<Rightarrow> 'x gensyn list \<Rightarrow> ('mstate \<Rightarrow> bool) \<Rightarrow> bool" 
   ("|_| {-_-} _ {-_-}")
   where
 "HT gs P c Q =
   (\<forall> c' .  |gs| {Q} (c') \<longrightarrow> |gs| {P} (c @ c'))"
+
+lemma HTI [intro] :
+  assumes H : "\<And> c' . |gs| {Q} (c') \<Longrightarrow> |gs| {P} (c @ c')"
+  shows "HT gs P c Q" using H unfolding HT_def
+  by auto
+
+lemma HTE [elim]:
+  assumes H : "HT gs P c Q"
+  assumes H' : "|gs| {Q} c'"
+  shows "|gs| {P} (c@c')" using assms
+  unfolding HT_def
+  by auto
 
 (* maybe there is another way we can achieve some kind of separation of concerns between control/continuation
    and the rest of the state... 
@@ -196,16 +238,12 @@ lemma HConseq :
    returning empty list vs returning None
    we could just not distinguish these cases.
 *)
-(*
-  or. another thought.
-*)
 lemma HStep : 
   assumes H : "(! sem ) % {{P}} c {{Q}}"
   assumes Hgs : "s_sem gs = sem"
   shows "|gs| {-P-} [G c l] {-Q-}" using H Hgs 
   unfolding HT_def guarded_def safe_def imm_safe_def semprop2_def VT_def 
   apply(auto)
-  apply(simp add: sem_exec_p_def)
 
   apply(drule_tac x = m in spec) apply(auto)
   apply(drule_tac x = "(s_sem gs c m) " in spec) apply(auto)
@@ -224,5 +262,97 @@ lemma HStep :
   apply(auto)
   done
 
+(* sequencing lemma *)
+lemma HCat :
+  assumes H : "|gs| {- P1 -} c1 {- P2 -}"
+  assumes H' : "|gs| {- P2 -} c2 {- P3 -}"
+  shows "|gs| {- P1 -} c1 @ c2 {- P3 -}"
+proof(rule HTI)
+  fix c'
+  assume HP3 : "|gs| {P3} c'"
+
+  have P2_cont : "|gs| {P2} c2 @ c'"
+    using HTE[OF H' HP3]
+    by auto
+
+  show "|gs| {P1} (c1 @ c2) @ c'"
+    using HTE[OF H P2_cont]
+    unfolding append_assoc
+    by auto
+qed
+
+definition determ :: "('a \<Rightarrow> 'a \<Rightarrow> bool) \<Rightarrow> bool" where
+"determ R \<equiv>
+  (\<forall> a b b' . R a b \<longrightarrow> R a b' \<longrightarrow> b = b')"
+
+lemma determI [intro] :
+  assumes "\<And> a b b' . R a b \<Longrightarrow> R a b' \<Longrightarrow> b = b'"
+  shows "determ R" using assms unfolding determ_def by auto
+
+lemma determE :
+  assumes H : "determ R"
+  assumes H1 : "R a b"
+  assumes H2 : "R a b'"
+  shows "b = b'" using assms
+  unfolding determ_def
+  by auto
+
+lemma sem_step_determ :
+  "determ (sem_step_p gs)"
+proof
+  fix a b b'
+  assume H1 : "sem_step_p gs a b"
+  assume H2 : "sem_step_p gs a b'"
+
+  show "b = b'" using H1 H2 unfolding sem_step_p_eq by auto
+qed
+
+(* helpful lemma for reasoning about compound executions *)
+lemma rtranclp_bisect1 :
+  assumes H0 : "determ R"
+  assumes H : "R\<^sup>*\<^sup>* xi xp"
+  assumes H1 : "R xi x1"
+  assumes H2 : "R xp xf"
+  shows "R\<^sup>*\<^sup>* x1 xf" using H H0 H1 H2
+proof(induction arbitrary: x1 xf rule: rtranclp_induct)
+  case base
+
+  have Eq : "x1 = xf" using determE[OF H0 base(2) base(3)] by auto
+
+  then show ?case using base by auto
+next
+  case (step y z)
+
+  have X1z : "R\<^sup>*\<^sup>* x1 z" using step.IH[OF step.prems(1) step.prems(2) step.hyps(2)]
+    by auto
+
+  show ?case using rtranclp.intros(2)[OF X1z step.prems(3)] by auto
+qed
+
+
+(*
+  Restriction requiring that predicates cannot look at continuation
+*)
+
+(*
+definition blind :: "('x, 'mstate) semc \<Rightarrow> ('mstate \<Rightarrow> bool) \<Rightarrow> bool" where
+"blind gs P =
+  (\<forall> x y . gs_cont x = gs_cont
+*)
+
+definition blind' :: "('x, 'mstate) semc \<Rightarrow> ('mstate \<Rightarrow> bool) \<Rightarrow> bool" where
+"blind' gs P =
+  (\<forall> c x . P x \<longrightarrow> (\<exists> x' . s_cont gs x' = c \<and> P x'))"
+
+lemma blind'E : 
+  assumes H : "blind' gs P"
+  assumes HP : "P x"
+  shows "\<exists> x' . s_cont gs x' = c \<and> P x'" using assms
+  unfolding blind'_def
+  by auto
+
+lemma blind'I [intro] :
+  assumes H : "(\<And> c x . P x \<Longrightarrow> (\<exists> x' . s_cont gs x' = c \<and> P x'))"
+  shows "blind' gs P" using H unfolding blind'_def by auto
 
 end
